RecordUpdate.v
@@ -1,0 +1,2 @@
+Require Export RecordSet.
+Export RecordSetNotations.
